Porting things up to the toplevel

src/coq/InterpreterMCFG.v
@@ -24,249 +24,291 @@ Section InterpreterMCFG.
    This gives us a _vertical_ notion of compositionality.
    *)
 
-  Definition interp_to_L1 {R} user_intrinsics (t: itree L0 R) g :=
+  Definition interp_to_L1 {R} user_intrinsics (t: itree L0 R) from :=
     let uvalue_trace       := interp_intrinsics user_intrinsics t in
-    let L1_trace           := interp_global uvalue_trace g in
+    let L1_trace           := interp_jmp uvalue_trace from in
     L1_trace.
 
-  Definition interp_to_L2 {R} user_intrinsics (t: itree L0 R) g l :=
-    let uvalue_trace   := interp_intrinsics user_intrinsics t in
-    let L1_trace       := interp_global uvalue_trace g in
-    let L2_trace       := interp_local_stack (handle_local (v:=uvalue)) L1_trace l in
+  Definition interp_to_L2 {R} user_intrinsics (t: itree L0 R) from g :=
+    let uvalue_trace       := interp_intrinsics user_intrinsics t in
+    let L1_trace           := interp_jmp uvalue_trace from in
+    let L2_trace           := interp_global L1_trace g in
     L2_trace.
 
-  Definition interp_to_L3 {R} user_intrinsics (t: itree L0 R) g l m :=
+  Definition interp_to_L3 {R} user_intrinsics (t: itree L0 R) from g l :=
     let uvalue_trace   := interp_intrinsics user_intrinsics t in
-    let L1_trace       := interp_global uvalue_trace g in
-    let L2_trace       := interp_local_stack (handle_local (v:=uvalue)) L1_trace l in
-    let L3_trace       := interp_memory L2_trace m in
+    let L1_trace       := interp_jmp uvalue_trace from in
+    let L2_trace       := interp_global L1_trace g in
+    let L3_trace       := interp_local_stack (handle_local (v:=uvalue)) L2_trace l in
     L3_trace.
 
-  Definition interp_to_L4 {R} RR user_intrinsics (t: itree L0 R) g l m :=
+  Definition interp_to_L4 {R} user_intrinsics (t: itree L0 R) from g l m :=
     let uvalue_trace   := interp_intrinsics user_intrinsics t in
-    let L1_trace       := interp_global uvalue_trace g in
-    let L2_trace       := interp_local_stack (handle_local (v:=uvalue)) L1_trace l in
-    let L3_trace       := interp_memory L2_trace m in
-    let L4_trace       := model_undef RR L3_trace in
+    let L1_trace       := interp_jmp uvalue_trace from in
+    let L2_trace       := interp_global L1_trace g in
+    let L3_trace       := interp_local_stack (handle_local (v:=uvalue)) L2_trace l in
+    let L4_trace       := interp_memory L3_trace m in
     L4_trace.
 
-  Definition interp_to_L5 {R} RR user_intrinsics (t: itree L0 R) g l m :=
+  Definition interp_to_L5 {R} RR user_intrinsics (t: itree L0 R) from g l m :=
     let uvalue_trace   := interp_intrinsics user_intrinsics t in
-    let L1_trace       := interp_global uvalue_trace g in
-    let L2_trace       := interp_local_stack (handle_local (v:=uvalue)) L1_trace l in
-    let L3_trace       := interp_memory L2_trace m in
-    let L4_trace       := model_undef RR L3_trace in
-    model_UB RR L4_trace.
+    let L1_trace       := interp_jmp uvalue_trace from in
+    let L2_trace       := interp_global L1_trace g in
+    let L3_trace       := interp_local_stack (handle_local (v:=uvalue)) L2_trace l in
+    let L4_trace       := interp_memory L3_trace m in
+    let L5_trace       := model_undef RR L4_trace in
+    L5_trace.
+
+  Definition interp_to_L6 {R} RR user_intrinsics (t: itree L0 R) from g l m :=
+    let uvalue_trace   := interp_intrinsics user_intrinsics t in
+    let L1_trace       := interp_jmp uvalue_trace from in
+    let L2_trace       := interp_global L1_trace g in
+    let L3_trace       := interp_local_stack (handle_local (v:=uvalue)) L2_trace l in
+    let L4_trace       := interp_memory L3_trace m in
+    let L5_trace       := model_undef RR L4_trace in
+    model_UB RR L5_trace.
 
   (* The interpreter stray away from the model starting from the fourth layer: we pick an arbitrary valid path of execution *)
-  Definition interp_to_L4_exec {R} user_intrinsics (t: itree L0 R) g l m :=
+  Definition interp_to_L5_exec {R} user_intrinsics (t: itree L0 R) from g l m :=
     let uvalue_trace   := interp_intrinsics user_intrinsics t in
-    let L1_trace       := interp_global uvalue_trace g in
-    let L2_trace       := interp_local_stack (handle_local (v:=uvalue)) L1_trace l in
-    let L3_trace       := interp_memory L2_trace m in
-    let L4_trace       := exec_undef L3_trace in
-    L4_trace.
+    let L1_trace       := interp_jmp uvalue_trace from in
+    let L2_trace       := interp_global L1_trace g in
+    let L3_trace       := interp_local_stack (handle_local (v:=uvalue)) L2_trace l in
+    let L4_trace       := interp_memory L3_trace m in
+    let L5_trace       := exec_undef L4_trace in
+    L5_trace.
 
-  Definition interp_to_L5_exec {R} user_intrinsics (t: itree L0 R) g l m :=
+  Definition interp_to_L6_exec {R} user_intrinsics (t: itree L0 R) from g l m :=
     let uvalue_trace   := interp_intrinsics user_intrinsics t in
-    let L1_trace       := interp_global uvalue_trace g in
-    let L2_trace       := interp_local_stack (handle_local (v:=uvalue)) L1_trace l in
-    let L3_trace       := interp_memory L2_trace m in
-    let L4_trace       := exec_undef L3_trace in
-    exec_UB L4_trace.
+    let L1_trace       := interp_jmp uvalue_trace from in
+    let L2_trace       := interp_global L1_trace g in
+    let L3_trace       := interp_local_stack (handle_local (v:=uvalue)) L2_trace l in
+    let L4_trace       := interp_memory L3_trace m in
+    let L5_trace       := exec_undef L4_trace in
+    exec_UB L5_trace.
 
   Section Structural_Lemmas.
 
-    Lemma interp_to_L1_bind :
-      forall ui {R S} (t: itree L0 R) (k: R -> itree L0 S) g, 
-        interp_to_L1 ui (ITree.bind t k) g ≈
-                     (ITree.bind (interp_to_L1 ui t g) (fun '(g',x) => interp_to_L1 ui (k x) g')).
-    Proof.
-      intros.
-      unfold interp_to_L1.
-      rewrite interp_intrinsics_bind, interp_global_bind.
-      apply eutt_eq_bind; intros (? & ?); reflexivity.
-    Qed.
+  Lemma interp_to_L1_bind :
+    forall ui {R S} (t: itree L0 R) (k: R -> itree L0 S) from, 
+      interp_to_L1 ui (ITree.bind t k) from ≈
+                       (ITree.bind (interp_to_L1 ui t from) (fun '(from',x) => interp_to_L1 ui (k x) from')).
+  Proof.
+    intros.
+    unfold interp_to_L1.
+    rewrite interp_intrinsics_bind, interp_jmp_bind.
+    apply eutt_eq_bind; intros (? & ?); reflexivity.
+  Qed.
 
-    Lemma interp_to_L1_ret : forall ui (R : Type) g (x : R), interp_to_L1 ui (Ret x) g ≈ Ret (g,x).
-    Proof.
-      intros; unfold interp_to_L1.
-      rewrite interp_intrinsics_ret, interp_global_ret; reflexivity.
-    Qed.
+  Lemma interp_to_L1_ret : forall ui (R : Type) from (x : R), interp_to_L1 ui (Ret x) from ≈ Ret (from,x).
+  Proof.
+    intros; unfold interp_to_L1.
+    rewrite interp_intrinsics_ret, interp_jmp_ret; reflexivity.
+  Qed.
+  
+  Lemma interp_to_L2_bind :
+    forall ui {R S} (t: itree L0 R) (k: R -> itree L0 S) from g, 
+      interp_to_L2 ui (ITree.bind t k) from g ≈
+      (ITree.bind (interp_to_L2 ui t from g) (fun '(g',(from',x)) => interp_to_L2 ui (k x) from' g')).
+  Proof.
+    intros.
+    unfold interp_to_L2.
+    rewrite interp_intrinsics_bind, interp_jmp_bind, interp_global_bind.
+    apply eutt_eq_bind; intros (? & ? & ?); reflexivity.
+  Qed.
 
-    Lemma interp_to_L2_bind :
-      forall ui {R S} (t: itree L0 R) (k: R -> itree L0 S) g l,
-        interp_to_L2 ui (ITree.bind t k) g l ≈
-                     (ITree.bind (interp_to_L2 ui t g l) (fun '(g',(l',x)) => interp_to_L2 ui (k x) l' g')).
-    Proof.
-      intros.
-      unfold interp_to_L2.
-      rewrite interp_intrinsics_bind, interp_global_bind, interp_local_stack_bind.
-      apply eutt_eq_bind; intros (? & ? & ?); reflexivity.
-    Qed.
+  Lemma interp_to_L2_ret : forall ui (R : Type) from g (x : R), interp_to_L2 ui (Ret x) from g ≈ Ret (g,(from,x)).
+  Proof.
+    intros; unfold interp_to_L2.
+    rewrite interp_intrinsics_ret, interp_jmp_ret, interp_global_ret; reflexivity.
+  Qed.
 
-    Lemma interp_to_L2_ret : forall ui (R : Type) g l (x : R), interp_to_L2 ui (Ret x) g l ≈ Ret (l, (g, x)).
-    Proof.
-      intros; unfold interp_to_L2.
-      rewrite interp_intrinsics_ret, interp_global_ret, interp_local_stack_ret; reflexivity.
-    Qed.
+  Lemma interp_to_L3_bind :
+    forall ui {R S} (t: itree L0 R) (k: R -> itree L0 S) from g l,
+      interp_to_L3 ui (ITree.bind t k) from g l ≈
+      (ITree.bind (interp_to_L3 ui t from g l) (fun '(l',(g',(from',x))) => interp_to_L3 ui (k x) from' g' l')).
+  Proof.
+    intros.
+    unfold interp_to_L3.
+    rewrite interp_intrinsics_bind, interp_jmp_bind, interp_global_bind, interp_local_stack_bind.
+    apply eutt_eq_bind; intros (? & ? & ? & ?); reflexivity.
+  Qed.
 
-    Lemma interp_to_L3_bind :
-      forall ui {R S} (t: itree L0 R) (k: R -> itree L0 S) g l m,
-        interp_to_L3 ui (ITree.bind t k) g l m ≈
-                     (ITree.bind (interp_to_L3 ui t g l m) (fun '(m',(l',(g',x))) => interp_to_L3 ui (k x) g' l' m')).
-    Proof.
-      intros.
-      unfold interp_to_L3.
-      rewrite interp_intrinsics_bind, interp_global_bind, interp_local_stack_bind, interp_memory_bind.
-      apply eutt_eq_bind; intros (? & ? & ? & ?); reflexivity.
-    Qed.
+  Lemma interp_to_L3_ret : forall ui (R : Type) from g l (x : R),
+      interp_to_L3 ui (Ret x) from g l ≈ Ret (l, (g, (from,x))).
+  Proof.
+    intros; unfold interp_to_L3.
+    rewrite interp_intrinsics_ret, interp_jmp_ret, interp_global_ret, interp_local_stack_ret; reflexivity.
+  Qed.
 
-    Lemma interp_to_L3_ret : forall ui (R : Type) g l m (x : R), interp_to_L3 ui (Ret x) g l m ≈ Ret (m, (l, (g,x))).
-    Proof.
-      intros; unfold interp_to_L3.
-      rewrite interp_intrinsics_ret, interp_global_ret, interp_local_stack_ret, interp_memory_ret; reflexivity.
-    Qed.
+  Lemma interp_to_L4_bind :
+    forall ui {R S} (t: itree L0 R) (k: R -> itree L0 S) from g l m,
+      interp_to_L4 ui (ITree.bind t k) from g l m ≈
+      (ITree.bind (interp_to_L4 ui t from g l m) (fun '(m',(l',(g',(from',x)))) => interp_to_L4 ui (k x) from' g' l' m')).
+  Proof.
+    intros.
+    unfold interp_to_L4.
+    rewrite interp_intrinsics_bind, interp_jmp_bind, interp_global_bind, interp_local_stack_bind, interp_memory_bind.
+    apply eutt_eq_bind; intros (? & ? & ? & ? & ?); reflexivity.
+  Qed.
 
-    Global Instance eutt_interp_to_L1 (defs: intrinsic_definitions) {T}:
-      Proper (eutt Logic.eq ==> Logic.eq ==> eutt Logic.eq) (@interp_to_L1 T defs).
-    Proof.
-      repeat intro.
-      unfold interp_to_L1.
-      subst; rewrite H.
-      reflexivity.
-    Qed.
+  Lemma interp_to_L4_ret :
+    forall ui (R : Type) from g l m (x : R),
+      interp_to_L4 ui (Ret x) from g l m ≈ Ret (m, (l, (g,(from,x)))).
+  Proof.
+    intros; unfold interp_to_L4.
+    rewrite interp_intrinsics_ret, interp_jmp_ret, interp_global_ret, interp_local_stack_ret, interp_memory_ret; reflexivity.
+  Qed.
 
-    Global Instance eutt_interp_to_L2 (defs: intrinsic_definitions) {T}:
-      Proper (eutt Logic.eq ==> Logic.eq ==> Logic.eq ==> eutt Logic.eq) (@interp_to_L2 T defs).
-    Proof.
-      repeat intro.
-      unfold interp_to_L2.
-      subst; rewrite H.
-      reflexivity.
-    Qed.
+  Global Instance eutt_interp_to_L1 (defs: intrinsic_definitions) {T}:
+    Proper (eutt Logic.eq ==> Logic.eq ==> eutt Logic.eq) (@interp_to_L1 T defs).
+  Proof.
+    repeat intro.
+    unfold interp_to_L1.
+    subst; rewrite H.
+    reflexivity.
+  Qed.
 
-    Global Instance eutt_interp_to_L3 (defs: intrinsic_definitions) {T}:
-      Proper (eutt Logic.eq ==> Logic.eq ==> Logic.eq ==> Logic.eq ==> eutt Logic.eq) (@interp_to_L3 T defs).
-    Proof.
-      repeat intro.
-      unfold interp_to_L3.
-      subst; rewrite H.
-      reflexivity.
-    Qed.
+  Global Instance eutt_interp_to_L2 (defs: intrinsic_definitions) {T}:
+    Proper (eutt Logic.eq ==> Logic.eq ==> Logic.eq ==> eutt Logic.eq) (@interp_to_L2 T defs).
+  Proof.
+    repeat intro.
+    unfold interp_to_L2.
+    subst; rewrite H.
+    reflexivity.
+  Qed.
 
-    (* NOTEYZ: This can probably be refined to [eqit eq] instead of [eutt eq], but I don't think it matters to us *)
-    Lemma interp_to_L3_vis (defs: IS.intrinsic_definitions):
-      forall T R (e : L0 T) (k : T -> itree L0 R) g l m,
-        interp_to_L3 defs (Vis e k) g l m ≈ 
-                     ITree.bind (interp_to_L3 defs (trigger e) g l m)
-                     (fun '(m, (l, (g, x)))=> interp_to_L3 defs (k x) g l m).
-    Proof.
-      intros.
-      unfold interp_to_L3.
-      rewrite interp_intrinsics_vis.
-      rewrite interp_global_bind, interp_local_stack_bind, interp_memory_bind.
-      unfold trigger; rewrite interp_intrinsics_vis.
-      rewrite interp_global_bind, interp_local_stack_bind, interp_memory_bind.
-      rewrite Eq.bind_bind.
-      apply eutt_eq_bind.
-      intros (? & ? & ? & ?).
-      do 2 match goal with
-             |- context[interp ?x ?t] => replace (interp x t) with (interp_intrinsics defs t) by reflexivity
-           end. 
-      rewrite interp_intrinsics_ret, interp_global_ret, interp_local_stack_ret, interp_memory_ret, bind_ret_l.
-      reflexivity.
-    Qed.
+  Global Instance eutt_interp_to_L3 (defs: intrinsic_definitions) {T}:
+    Proper (eutt Logic.eq ==> Logic.eq ==> Logic.eq ==> Logic.eq ==> eutt Logic.eq) (@interp_to_L3 T defs).
+  Proof.
+    repeat intro.
+    unfold interp_to_L3.
+    subst; rewrite H.
+    reflexivity.
+  Qed.
 
-    Lemma interp_to_L3_bind_trigger (defs: IS.intrinsic_definitions):
-      forall T R (e : L0 T) (k : T -> itree L0 R) g l m,
-        interp_to_L3 defs (ITree.bind (trigger e) k) g l m ≈ 
-                     ITree.bind (interp_to_L3 defs (trigger e) g l m)
-                     (fun '(m, (l, (g, x)))=> interp_to_L3 defs (k x) g l m).
-    Proof.
-      intros.
-      rewrite bind_trigger.
-      rewrite interp_to_L3_vis at 1.
-      reflexivity.
-    Qed.
+  Global Instance eutt_interp_to_L4 (defs: intrinsic_definitions) {T}:
+    Proper (eutt Logic.eq ==> Logic.eq ==> Logic.eq ==> Logic.eq ==> Logic.eq ==> eutt Logic.eq) (@interp_to_L4 T defs).
+  Proof.
+    repeat intro.
+    unfold interp_to_L4.
+    subst; rewrite H.
+    reflexivity.
+  Qed.
 
-    Lemma interp_to_L3_GW : forall defs id g l m v,
-        interp_to_L3 defs (trigger (GlobalWrite id v)) g l m ≈ ret (m,(l,(Maps.add id v g,tt))).
-    Proof.
-      intros.
-      unfold interp_to_L3.
-      rewrite interp_intrinsics_trigger; cbn. 
-      unfold Intrinsics.F_trigger.
-      rewrite interp_global_trigger; cbn.
-      unfold interp_local_stack.
-      rewrite interp_state_ret, interp_memory_ret.
-      reflexivity.
-    Qed.
+  Lemma interp_to_L4_vis (defs: IS.intrinsic_definitions):
+    forall T R (e : L0 T) (k : T -> itree L0 R) from g l m,
+      interp_to_L4 defs (Vis e k) from g l m ≈ 
+                   ITree.bind (interp_to_L4 defs (trigger e) from g l m)
+                   (fun '(m, (l, (g, (from, x))))=> interp_to_L4 defs (k x) from g l m).
+  Proof.
+    intros.
+    unfold interp_to_L4.
+    rewrite interp_intrinsics_vis.
+    rewrite interp_jmp_bind,interp_global_bind, interp_local_stack_bind, interp_memory_bind.
+    unfold trigger; rewrite interp_intrinsics_vis.
+    rewrite interp_jmp_bind, interp_global_bind, interp_local_stack_bind, interp_memory_bind.
+    rewrite Eq.bind_bind.
+    apply eutt_eq_bind.
+    intros (? & ? & ? & ? & ?).
+    do 2 match goal with
+           |- context[interp ?x ?t] => replace (interp x t) with (interp_intrinsics defs t) by reflexivity
+         end. 
+    rewrite interp_intrinsics_ret, interp_jmp_ret, interp_global_ret, interp_local_stack_ret, interp_memory_ret, bind_ret_l.
+    reflexivity.
+  Qed.
 
-    Lemma interp_cfg_to_L3_LM : forall defs t a size offset g l m v bytes concrete_id,
-        get_logical_block m a = Some (LBlock size bytes concrete_id) ->
-        deserialize_sbytes (lookup_all_index offset (sizeof_dtyp t) bytes SUndef) t = v ->
-        interp_to_L3 defs (trigger (Load t (DVALUE_Addr (a, offset)))) g l m ≈ Ret (m,(l,(g,v))).
-    Proof.
-      intros * LUL EQ.
-      unfold interp_to_L3.
-      rewrite interp_intrinsics_trigger.
-      cbn.
-      unfold Intrinsics.F_trigger.
-      rewrite interp_global_trigger.
-      cbn.
-      unfold interp_local_stack.
-      rewrite interp_state_bind.
-      rewrite interp_state_trigger.
-      cbn. rewrite bind_bind.
-      rewrite bind_trigger.
-      rewrite interp_memory_vis.
-      cbn.
-      destruct m as [mem memstack]. cbn.
-      cbn in LUL. unfold read.
-      cbn; rewrite LUL.
-      cbn; rewrite 2 bind_ret_l.
-      rewrite interp_state_ret.
-      rewrite interp_memory_ret.
-      cbn in *.
-      unfold read_in_mem_block. rewrite EQ.
-      reflexivity.
-    Qed.
+  Lemma interp_to_L4_bind_trigger (defs: IS.intrinsic_definitions):
+    forall T R (e : L0 T) (k : T -> itree L0 R) from g l m,
+      interp_to_L4 defs (ITree.bind (trigger e) k) from g l m ≈ 
+                   ITree.bind (interp_to_L4 defs (trigger e) from g l m)
+                   (fun '(m, (l, (g, (from, x))))=> interp_to_L4 defs (k x) from g l m).
+  Proof.
+    intros.
+    rewrite bind_trigger.
+    rewrite interp_to_L4_vis at 1.
+    reflexivity.
+  Qed.
 
-    Lemma interp_to_L3_alloca :
-      forall (defs : intrinsic_definitions) (m : memory_stack) (t : dtyp) (g : global_env) l,
-        non_void t ->
-        exists m' a',
-          allocate m t = inr (m', a') /\
-          interp_to_L3 defs (trigger (Alloca t)) g l m ≈ ret (m', (l, (g, DVALUE_Addr a'))).
-    Proof.
-      intros * NV.
-      unfold interp_to_L3.
-      eapply interp_memory_alloca_exists in NV as [m' [a' [ALLOC INTERP]]].
-      exists m'. exists a'.
+  Lemma interp_to_L4_GW : forall defs id from g l m v,
+      interp_to_L4 defs (trigger (GlobalWrite id v)) from g l m ≈ ret (m,(l,(Maps.add id v g,(from,tt)))).
+  Proof.
+    intros.
+    unfold interp_to_L4.
+    rewrite interp_intrinsics_trigger; cbn. 
+    unfold Intrinsics.F_trigger.
+    rewrite interp_jmp_trigger; cbn.
+    rewrite subevent_subevent.
+    rewrite interp_global_bind,interp_global_trigger; cbn.
+    rewrite bind_ret_l, interp_global_ret, interp_local_stack_ret, interp_memory_ret.
+    reflexivity.
+  Qed.
+  (* TODO: Redo this proof, it has no business unfolding so much *)
+  Lemma interp_cfg_to_L4_LM : forall defs t a size offset from g l m v bytes concrete_id,
+      get_logical_block m a = Some (LBlock size bytes concrete_id) ->
+      deserialize_sbytes (lookup_all_index offset (sizeof_dtyp t) bytes SUndef) t = v ->
+      interp_to_L4 defs (trigger (Load t (DVALUE_Addr (a, offset)))) from g l m ≈ Ret (m,(l,(g,(from,v)))).
+  Proof.
+    intros * LUL EQ.
+    unfold interp_to_L4.
+    rewrite interp_intrinsics_trigger.
+    cbn.
+    unfold Intrinsics.F_trigger.
+    rewrite interp_jmp_trigger; cbn; rewrite subevent_subevent.
+    rewrite interp_global_bind,interp_global_trigger.
+    cbn; rewrite subevent_subevent.
+    rewrite bind_bind, interp_local_stack_bind.
+    unfold interp_local_stack.
+    rewrite interp_state_trigger; cbn; rewrite subevent_subevent.
+    rewrite bind_bind.
+    rewrite bind_trigger.
+    rewrite interp_memory_vis.
+    cbn.
+    destruct m as [mem memstack]. cbn.
+    cbn in LUL. unfold read.
+    cbn; rewrite LUL.
+    cbn; repeat rewrite bind_ret_l.
+    cbn.
+    rewrite interp_global_ret, interp_state_ret, interp_memory_ret.
+    cbn in *.
+    unfold read_in_mem_block. rewrite EQ.
+    reflexivity.
+  Qed.
 
-      rewrite interp_intrinsics_trigger.
-      cbn.
-      unfold Intrinsics.F_trigger.
-      rewrite interp_global_trigger.
-      cbn.
-      unfold interp_local_stack.
-      rewrite interp_state_bind.
-      rewrite interp_state_trigger.
-      cbn.
-      rewrite bind_bind.
-      rewrite interp_memory_bind.
-      rewrite subevent_subevent, interp_memory_alloca; eauto.
-      cbn.
-      repeat rewrite bind_ret_l.
-      cbn.
-      rewrite interp_state_ret.
-      rewrite interp_memory_ret.
-      split; eauto.
-      reflexivity.
-      Unshelve.
-      auto.
-    Qed.
+  Lemma interp_to_L4_alloca :
+    forall (defs : intrinsic_definitions) (m : memory_stack) (t : dtyp) from (g : global_env) l,
+      non_void t ->
+      exists m' a',
+        allocate m t = inr (m', a') /\
+        interp_to_L4 defs (trigger (Alloca t)) from g l m ≈ ret (m', (l, (g, (from, DVALUE_Addr a')))).
+  Proof.
+    intros * NV.
+    unfold interp_to_L4.
+    eapply interp_memory_alloca_exists in NV as [m' [a' [ALLOC INTERP]]].
+    exists m'. exists a'.
+
+    rewrite interp_intrinsics_trigger.
+    cbn.
+    unfold Intrinsics.F_trigger.
+    rewrite interp_jmp_trigger; cbn; rewrite subevent_subevent.
+    rewrite interp_global_bind, interp_global_trigger.
+    cbn; rewrite bind_bind.
+    unfold interp_local_stack.
+    rewrite interp_state_bind.
+    rewrite interp_state_trigger.
+    cbn.
+    rewrite bind_bind.
+    rewrite interp_memory_bind.
+    rewrite subevent_subevent, interp_memory_alloca; eauto.
+    cbn.
+    repeat rewrite bind_ret_l.
+    cbn.
+    rewrite interp_global_ret, interp_state_ret, interp_memory_ret.
+    split; eauto.
+    reflexivity.
+    Unshelve.
+    auto.
+  Qed.
 
   End Structural_Lemmas.
 
